Switch to a function for the incremental ghost API, following discussions with Nik. Document the discussions as comments in the code. Update the implementation. Fix hopefully the last fragile proof in this module with another very explicit proof.3

providers/evercrypt/EverCrypt.Hash.Incremental.fsti
@@ -50,6 +50,7 @@ let any_hash_t_fits (a: alg) (b: any_hash_t): Lemma
   ()
 #pop-options
 
+
 /// Abstract footprints, with the same machinery as EverCrypt.Hash
 /// --------------------------------------------------------------
 ///
@@ -97,19 +98,57 @@ val invariant_loc_in_footprint
 /// ----------------------------------------
 ///
 /// We offer a stateful predicate that allows the client to tie a particular
-/// state to a sequence of bytes hashed so far.
+/// state to a sequence of bytes hashed so far. There are a variety of styles
+/// possible, here's a recap and a discussion of the respective merits of each
+/// style, so that we document and avoid going back and forth for future APIs.
+///
+/// 1. val update (b: erased bytes): unit
+///      requires (fun h0 -> hashes h0 s b)
+///      ensures (fun h1 -> hashes h1 s (b `append` data))
+///
+///    The problem with this one is that it requires the client to not only
+///    explicitly pass an erased argument, but also requires the client, when
+///    chaining calls to construct the "next" value by manually concatenating
+///    (ghostly) bytes.
+///
+/// 2. val update (b: erased bytes): erased bytes
+///      requires (fun h0 -> hashes h0 s b)
+///      ensures (fun h1 b' -> hashes h1 s b' /\ b' == b `append` data)
+///
+///    This one is a slight improvement over 1. because the client can "get
+///    their hands" on the returned bytes and doesn't need to manually create
+///    the concatenation ``b `append` data`` when they chain another call to
+///    update.
+///
+/// 3. val update (): unit
+///      requires _
+///      ensures (fun h0 _ h1 -> hashed h1 s == hashed h0 s `append` data)
+///
+///    While 1. and 2. were based on a predicate, this one relies on a function
+///    that returns the bytes (ghostly) for any given state and heap. It does
+///    not require the client to materialize the erased bytes, and it does not
+///    require the client to manually construct intermediary ghost byte values
+///    when chaining.
+///
+/// 4. There's another style based on a state machine and an erased value that
+///    materializes all the ghost state in a single record, thus requiring only a
+///    single framing lemma (as opposed to three or more for the styles 1. 2. and
+///    3.). It appears that this may be overkill for this module and may be better
+///    suited to TLS.
+///                                            JP (20190607)
 
 noextract
 let bytes = S.seq UInt8.t
 
-val hashes: #a:Hash.alg -> h:HS.mem -> s:state a -> b:bytes -> Type0
+val hashed: #a:Hash.alg -> h:HS.mem -> s:state a -> GTot bytes
 
 // This should alleviate the need for painful proofs about things fitting.
-val hash_fits: #a:Hash.alg -> h:HS.mem -> s:state a -> b:bytes -> Lemma
-  (requires hashes h s b)
+val hash_fits: #a:Hash.alg -> h:HS.mem -> s:state a -> Lemma
+  (requires (
+    invariant h s))
   (ensures (
-    S.length b < Spec.Hash.Definitions.max_input_length a))
-  [ SMTPat (hashes h s b) ]
+    S.length (hashed h s) < Spec.Hash.Definitions.max_input_length a))
+  [ SMTPat (hashed h s) ]
 
 
 /// Central frame invariants
@@ -146,14 +185,15 @@ val frame_invariant: #a:alg -> l:B.loc -> s:state a -> h0:HS.mem -> h1:HS.mem ->
   (ensures (
     invariant h1 s /\
     footprint h0 s == footprint h1 s))
+  [ SMTPat (invariant h1 s); SMTPat (B.modifies l h0 h1) ]
 
-val frame_hashes: #a:alg -> l:B.loc -> s:state a -> b:bytes -> h0:HS.mem -> h1:HS.mem -> Lemma
+val frame_hashed: #a:alg -> l:B.loc -> s:state a -> h0:HS.mem -> h1:HS.mem -> Lemma
   (requires (
     invariant h0 s /\
-    hashes h0 s b /\
     B.loc_disjoint l (footprint h0 s) /\
     B.modifies l h0 h1))
-  (ensures (hashes h1 s b))
+  (ensures (hashed h0 s == hashed h1 s))
+  [ SMTPat (hashed h1 s); SMTPat (B.modifies l h0 h1) ]
 
 val frame_freeable: #a:alg -> l:B.loc -> s:state a -> h0:HS.mem -> h1:HS.mem -> Lemma
   (requires (
@@ -162,6 +202,7 @@ val frame_freeable: #a:alg -> l:B.loc -> s:state a -> h0:HS.mem -> h1:HS.mem -> 
     B.loc_disjoint l (footprint h0 s) /\
     B.modifies l h0 h1))
   (ensures (freeable h1 s))
+  [ SMTPat (freeable h1 s); SMTPat (B.modifies l h0 h1) ]
 
 /// Stateful API
 /// ------------
@@ -186,7 +227,7 @@ val init (a: Hash.alg) (s: state a): Stack unit
   (ensures (fun h0 _ h1 ->
     preserves_freeable s h0 h1 /\
     invariant h1 s /\
-    hashes h1 s S.empty /\
+    hashed h1 s == S.empty /\
     footprint h0 s == footprint h1 s /\
     B.(modifies (footprint h0 s) h0 h1)))
 
@@ -194,23 +235,20 @@ unfold
 let update_pre
   (a: Hash.alg)
   (s: state a)
-  (prev: G.erased bytes)
   (data: B.buffer UInt8.t)
   (len: UInt32.t)
   (h0: HS.mem)
 =
   invariant h0 s /\
-  hashes h0 s (G.reveal prev) /\
   B.live h0 data /\
   U32.v len = B.length data /\
-  S.length (G.reveal prev) + U32.v len < pow2 61 /\
+  S.length (hashed h0 s) + U32.v len < pow2 61 /\
   B.(loc_disjoint (loc_buffer data) (footprint h0 s))
 
 unfold
 let update_post
   (a: Hash.alg)
   (s: state a)
-  (prev: G.erased bytes)
   (data: B.buffer UInt8.t)
   (len: UInt32.t)
   (h0 h1: HS.mem)
@@ -219,40 +257,37 @@ let update_post
   invariant h1 s /\
   B.(modifies (footprint h0 s) h0 h1) /\
   footprint h0 s == footprint h1 s /\
-  hashes h1 s (Seq.append (G.reveal prev) (B.as_seq h0 data))
+  hashed h1 s == hashed h0 s `S.append` B.as_seq h0 data
 
 (** @type: true
 *)
 val update:
   a:Hash.alg ->
   s:state a ->
-  prev:G.erased bytes ->
   data: B.buffer UInt8.t ->
   len: UInt32.t ->
   Stack unit
-    (requires fun h0 -> update_pre a s prev data len h0)
-    (ensures fun h0 s' h1 -> update_post a s prev data len h0 h1)
+    (requires fun h0 -> update_pre a s data len h0)
+    (ensures fun h0 s' h1 -> update_post a s data len h0 h1)
 
 /// Note: the state is left to be reused by the caller to feed more data into
 /// the hash.
 inline_for_extraction
 let finish_st (a: Hash.alg) =
   s:state a ->
-  prev:G.erased bytes ->
   dst: Hacl.Hash.Definitions.hash_t a ->
   Stack unit
     (requires fun h0 ->
       invariant h0 s /\
-      hashes h0 s (G.reveal prev) /\
       B.live h0 dst /\
       B.(loc_disjoint (loc_buffer dst) (footprint h0 s)))
     (ensures fun h0 s' h1 ->
       preserves_freeable s h0 h1 /\
       invariant h1 s /\
-      hashes h1 s (G.reveal prev) /\
+      hashed h0 s == hashed h1 s /\
       footprint h0 s == footprint h1 s /\
       B.(modifies (loc_union (loc_buffer dst) (footprint h0 s)) h0 h1) /\
-      S.equal (B.as_seq h1 dst) (Spec.Hash.hash a (G.reveal prev)))
+      S.equal (B.as_seq h1 dst) (Spec.Hash.hash a (hashed h0 s)))
 
 (** @type: true
 *)
